Implementation of the calculus of substitution. Syntax could still be improve for redability. Notation seems not usefull as they are

Gratzer&Angiuli_Dependant_Types./Definitions.v
@@ -3,28 +3,456 @@ From Corelib.Program Require Import Basics Tactics Wf.
 From Stdlib.Logic Require Import JMeq.
 
 Require Export Setoid.
-Require Export Relation_Definitions.
 
+Require Export Relation_Definitions.
 (* Implementation of Dependent Types in Rocq (From Gratzer's "Principles of Dependent Type Theory") *)
 
-Inductive preType :=
-| Base : preType
-| Func (A B : preType) : preType
-| Prod (A B : preType) : preType.
+(** Syntax **)
 
-Notation "A --> B" := (Func A B) (at level 55,  right associativity).
-Notation "A ** B" := (Prod A B) (at level 60, right associativity).
+(** Pre-syntax definitions **)
 
-Inductive preContext : nat -> Type :=
-   Empty : preContext 0
-| Extend : forall{n}, preContext n -> preType -> preContext (S n).
+(** Convention For syntax sorts.
+   Contexts ctx: greek uppercase letters: Gamma, Delta, ...
+   Types t : uppercase letters: A, B, ...
+   Terms e : lowercase letters: a, b, ...
+   Substitutions g :  indexed g : g0, g1, ...
+**)
 
-Notation "ctx # A" := (Extend ctx A) (at level 50, left associativity).
+Inductive preContext : Set :=
+  One : preContext
+| CExt: preContext -> preType -> preContext
+with preSub : Set :=
+| Id : preContext -> preSub
+| Weak : preContext -> preType -> preSub
+| Comp : preSub -> preSub -> preSub
+(** Terminal subst **)
+| Bang : preContext -> preSub
+(** Extension **)
+| SExt : preContext
+   -> preContext -> preSub
+   -> preType -> preTerm
+   -> preSub
+with preType : Set :=
+| Base : preContext -> preType
+| Func : preContext -> preType -> preType -> preType
+| Prod : preContext -> preType -> preType -> preType
+| TSubst : preContext -> preType -> preSub -> preType
+with preTerm : Set :=
+| Qar : (preContext * preType) -> preTerm
+| Const : preContext -> nat -> preTerm
+| Pair :  preContext
+   -> preType -> preTerm
+   -> preType -> preTerm
+   -> preTerm
+| Fst : preContext
+   -> preType * preType -> preTerm
+   -> preTerm
+| Snd : preContext
+   -> preType * preType -> preTerm
+   -> preTerm
+| Lam : preContext
+   -> preType
+   -> preType -> preTerm
+   -> preTerm
+| App : preContext
+   -> preType -> preTerm
+   -> preType -> preTerm
+   -> preTerm
+| ESubst : preContext
+   -> preType -> preTerm
+   -> preContext -> preSub
+   -> preTerm
+.
 
-Inductive preTerm :=
-| const (n : nat) : preTerm
-| Pair (a b : preTerm) : preTerm
-| Fst (p : preTerm) : preTerm
-| Snd (p : preTerm) : preTerm
-| Lam (b : preTerm) : preTerm
-| App (f a : preTerm) : preTerm.
+Scheme preContext_Type_rec := Induction for preContext Sort Set
+   with preType_Context_rec := Induction for preType Sort Set.
+
+About preContext_Type_rec.
+
+Scheme preSub_Context_rec := Induction for preSub Sort Set
+   with preContext_Sub_rec := Induction for preTerm Sort Set.
+About preSub_Context_rec.
+
+Scheme preType_Context_Sub_rec := Induction for preType Sort Set
+   with preContext_Sub_Type_rec := Induction for preContext Sort Set
+   with preSub_Type_Context_rec := Induction for preSub Sort Set.
+About preType_Context_Sub_rec.
+
+Scheme preTerm_Context_Sub_Type_rec := Induction for preTerm Sort Set
+   with preContext_Sub_Type_Term_rec := Induction for preContext Sort Set
+   with preSub_Type_Term_Context_rec := Induction for preSub Sort Set
+   with preType_Term_Context_Sub_rec := Induction for preType Sort Set.
+About preTerm_Context_Sub_Type_rec.
+
+Notation "ctx ,c A" := (CExt ctx A) (at level 50, left associativity).
+
+Notation "A --> B" := (Func _ A B) (at level 55,  right associativity).
+Notation "A ** B" := (Prod _ A B) (at level 60, right associativity).
+
+Notation "A '[t' g ]" := (TSubst _ A g) (at level 50).
+Notation "a '[e' g ]" := (ESubst _ a g) (at level 50).
+
+(* Notation "g ,s a " := (SExt g a) (at level 50). *)
+
+(** Syntax Jugements *)
+
+Fixpoint ContextJG (ctx : preContext) {struct ctx} : Prop :=
+  match ctx with
+  | One => True
+  | CExt Gamma A => ContextJG Gamma /\ TypeJG Gamma A
+  end
+  with
+   SubsJG (Delta : preContext) (g : preSub) (Gamma : preContext) {struct g} : Prop :=
+  (* Presupose *)
+  match g with
+   | Id ctx => Delta = ctx /\ ctx = Gamma /\ ContextJG ctx
+   | Weak ctx A => Delta = ctx ,c A /\ ctx = Gamma /\ ContextJG ctx /\ TypeJG ctx A
+   | Comp g0 g1 =>
+       exists ctx1,
+       (* Delta = ctx2, Gamma = ctx0 *)
+       SubsJG Delta g1 ctx1 /\
+       SubsJG ctx1 g0 Gamma
+   | Bang ctx => Delta = ctx /\Gamma = One /\ ContextJG ctx
+   | SExt ctx ctx' g A a =>
+         ctx = Delta /\ ContextJG ctx /\
+         Gamma = ctx',c A /\ ContextJG ctx' /\
+         SubsJG Delta g ctx' /\
+         TypeJG ctx' A /\
+         TermJG ctx (TSubst ctx' A g) a
+  end
+
+  with TypeJG (ctx : preContext) (A : preType) {struct A} : Prop :=
+   match A with
+   | Base Gamma => Gamma = ctx /\ ContextJG Gamma
+   | Func Gamma A1 A2 =>
+      Gamma = ctx /\ ContextJG Gamma /\
+       TypeJG ctx A1 /\ TypeJG ctx A2
+   | Prod Gamma A1 A2 =>
+      Gamma = ctx /\ ContextJG Gamma /\
+       TypeJG ctx A1 /\ TypeJG ctx A2
+   | TSubst Gamma A g =>
+         Gamma = ctx /\ ContextJG Gamma /\
+         TypeJG Gamma A /\
+         SubsJG ctx g Gamma
+   end
+
+  with TermJG (ctx : preContext) (ty : preType) (e : preTerm) {struct e} : Prop :=
+  match e with
+   | Qar (Gamma, A) => ContextJG Gamma /\ TypeJG Gamma A /\
+       ty = A /\ Gamma = ctx
+   | Const Gamma n => Gamma = ctx /\ ty = Base Gamma /\ ContextJG Gamma
+   | Pair Gamma A1 a A2 b =>
+       Gamma = ctx /\ ContextJG Gamma /\
+       TypeJG ctx A1 /\ TypeJG ctx A2 /\
+       ty = Prod ctx A1 A2 /\
+       TermJG ctx A1 a /\
+       TermJG ctx A2 b
+   | Fst Gamma (A,B) p =>
+       Gamma = ctx /\ ContextJG Gamma /\
+       ty = A /\ TypeJG ctx A /\ TypeJG ctx B /\
+       TermJG ctx (Prod ctx A B) p
+   | Snd Gamma (A,B) p =>
+       Gamma = ctx /\ ContextJG Gamma /\
+       ty = B /\ TypeJG ctx A /\ TypeJG ctx B /\
+       TermJG ctx (Prod ctx A B) p
+   | Lam Gamma A B b =>
+       Gamma = ctx /\ ContextJG Gamma /\
+         ty = Func ctx A B /\ TypeJG ctx A /\ TypeJG (ctx ,c A) B /\
+         TermJG (ctx ,c A) B b
+   | App Gamma A f B a =>
+       Gamma = ctx /\ ContextJG Gamma /\
+         ty = B /\ TypeJG ctx A /\ TypeJG (ctx ,c A) B /\
+         TermJG ctx (Func ctx A B) f /\
+         TermJG ctx A a
+   | ESubst Gamma B a Delta g =>
+       Gamma = ctx /\ ContextJG Gamma /\
+         ty = TSubst ctx B g /\ TypeJG Delta B /\
+         TermJG Delta B a /\
+         SubsJG Gamma g Delta
+   end
+  .
+
+Notation "[ ⊢ ctx ]" := (ContextJG ctx) (at level 50).
+Notation "[ Delta ⊢ g :s Gamma ]" := (SubsJG Delta g Gamma) (at level 50).
+Notation "[ ctx ⊢ A ]" := (TypeJG ctx A) (at level 50).
+Notation "[ ctx ⊢ t ; A ]" := (TermJG ctx A t) (at level 50).
+
+(** End Syntax Judgements **)
+
+(* Example Judgements *)
+Example ex1 :
+   let B := Base One in
+   [ One ⊢ Func One (Prod One B B) B ].
+Proof.
+  repeat split.
+Qed.
+
+(** Well-formed syntax types **)
+
+Inductive wfCtx : Type := {
+  ctx :> preContext;
+  ctx_judg : ContextJG ctx
+}.
+
+Inductive wfType (ctx : wfCtx) : Type := {
+  ty :> preType;
+  ty_judg : TypeJG ctx ty
+}.
+
+Definition wfOne : wfCtx.
+   refine ({|
+      ctx := One;
+      ctx_judg := _
+   |}).
+   constructor.
+Defined.
+Notation "1" := (wfOne).
+
+Definition wf_Ext {ctx : wfCtx} (A : @wfType ctx) : wfCtx.
+   refine ({|
+      ctx := ctx ,c A;
+      ctx_judg := _
+      |}).
+      destruct ctx as [ctx ctx_judg].
+      destruct A as [A A_judg].
+      simpl in *.
+      split; assumption.
+Defined.
+Notation "ctx ,c A" := (@wf_Ext ctx A) (at level 50, left associativity).
+Inductive wfSub {Delta Gamma : wfCtx}: Type := {
+  sub :> preSub;
+  sub_judg : SubsJG Delta sub Gamma
+}.
+
+Definition wf_Id {ctx : wfCtx} : @wfSub ctx ctx.
+   refine ({|
+      sub := Id ctx;
+      sub_judg := _
+   |}).
+   destruct ctx as [ctx ctx_judg].
+   simpl.
+   tauto.
+Defined.
+
+Definition proj {ctx : wfCtx} {A : @wfType ctx} : @wfSub (ctx ,c A) ctx.
+   refine ({|
+      sub := Weak ctx A;
+      sub_judg := _
+   |}).
+   destruct ctx as [ctx ctx_judg].
+   destruct A as [A A_judg].
+   simpl in *.
+   repeat split;
+   assumption.
+Defined.
+
+Inductive wfTerm (ctx : wfCtx) (A : wfType ctx) : Type := {
+  term :> preTerm;
+  term_judg : TermJG ctx A term
+}.
+
+(** End Well-formed syntax types **)
+
+Definition sub_compose
+   (Delta mid Gamma : wfCtx)
+   (g0 : @wfSub mid Gamma)
+   (g1 : @wfSub Delta mid) : @wfSub Delta Gamma.
+Proof.
+   refine ({|
+      sub := Comp g0 g1;
+      sub_judg := _
+   |}).
+   destruct g0 as [g0 H0].
+   destruct g1 as [g1 H1].
+   simpl.
+   exists mid.
+   split; assumption.
+Defined.
+Notation "gamma1 '∘' gamma2" := (sub_compose _ _ _ gamma1 gamma2) (at level 40, left associativity).
+
+
+(** Equality Judgements   **)
+
+(*** Equality of substitutions ***)
+Inductive eq_sub :  relation (preSub) :=
+(** Enforce equivalence **)
+| EqReflSub : forall gamma, eq_sub gamma gamma
+| EqSymSub : forall gamma1 gamma2,
+   eq_sub gamma1 gamma2 ->
+   eq_sub gamma2 gamma1
+| EqTransSub : forall gamma1 gamma2 gamma3,
+   eq_sub gamma1 gamma2 ->
+   eq_sub gamma2 gamma3 ->
+   eq_sub gamma1 gamma3
+(** Enforce compatibility with composition **)
+| EqLeftId : forall {Delta Gamma} (gamma : @wfSub Delta Gamma),
+   eq_sub (sub wf_Id ∘ gamma) (sub gamma)
+| EqRightId : forall {Delta Gamma} (gamma : @wfSub Delta Gamma),
+  eq_sub (sub gamma ∘ wf_Id) (sub gamma)
+| EqCompAssoc (ctx0 ctx1 ctx2 ctx3 : wfCtx) (gamma2 : @wfSub ctx3 ctx2) (gamma1 : @wfSub ctx2 ctx1) (gamma0 : @wfSub ctx1 ctx0):
+   eq_sub
+   (sub_compose ctx3 ctx1 ctx0 gamma0 (sub_compose ctx3 ctx2 ctx1 gamma1 gamma2))
+   (sub_compose ctx3 ctx2 ctx0 (sub_compose ctx2 ctx1 ctx0 gamma0 gamma1) gamma2)
+| EqCompSub : forall (gamma1 gamma1' gamma2 gamma2' : preSub),
+   eq_sub gamma1 gamma1' ->
+   eq_sub gamma2 gamma2' ->
+   eq_sub (Comp gamma1 gamma2) (Comp gamma1' gamma2')
+| EqBang : forall {Gamma} (g : @wfSub Gamma 1),
+   eq_sub (Bang Gamma) g
+.
+
+
+Definition SubsEqJG {delta : wfCtx} {ctx : wfCtx} : relation (@wfSub delta ctx) := eq_sub.
+
+Lemma SubsEqJG_refl {delta : wfCtx} {ctx : wfCtx} (gamma : @wfSub delta ctx) :
+    SubsEqJG gamma gamma.
+Proof.
+   constructor.
+Qed.
+
+Lemma SubsEqJG_sym {delta ctx : wfCtx} (gamma gamma' : @wfSub delta ctx) :
+   SubsEqJG gamma gamma'  ->
+   SubsEqJG gamma' gamma.
+Proof.
+   constructor.
+   exact H.
+Qed.
+   (* intros H.
+   unfold SubsEqJG in *.
+   induction H; subst; constructor.
+   all: assumption.
+Qed. *)
+
+Lemma SubsEqJG_trans {delta ctx : wfCtx} (gamma1 gamma2 gamma3 : @wfSub delta ctx) :
+   SubsEqJG gamma1 gamma2 ->
+   SubsEqJG gamma2 gamma3 ->
+   SubsEqJG gamma1 gamma3.
+Proof.
+   apply EqTransSub.
+Qed.
+
+Add Parametric Relation (delta ctx :wfCtx) : (@wfSub delta ctx) (@SubsEqJG delta ctx)
+   reflexivity proved by (@SubsEqJG_refl delta ctx)
+   symmetry proved by (@SubsEqJG_sym delta ctx)
+   transitivity proved by (@SubsEqJG_trans delta ctx)
+   as SubsEqJG_rel.
+
+Notation "[ Delta ⊢ g1 '==' g2 :s Gamma ]" := (@SubsEqJG Delta Gamma g1 g2) (at level 50).
+
+Add Parametric Morphism (Delta mid Gamma : wfCtx) : (@sub_compose Delta mid Gamma)
+   with signature (@SubsEqJG mid Gamma  ==> @SubsEqJG Delta mid ==> @SubsEqJG Delta Gamma)
+   as SubsEqJG_mor.
+Proof.
+   unfold SubsEqJG in *.
+   simpl.
+   intros gamma1 gamma2 H12.
+   intros gamma1' gamma2' H12'.
+   apply EqCompSub; assumption.
+Qed.
+
+
+(*** End Equality of substitutions ***)
+
+(*** Equality for Types ***)
+Inductive eq_type : relation preType :=
+(** Enforce equivalence **)
+| EqReflType : forall A, eq_type A A
+| EqSymType : forall A1 A2,
+   eq_type A1 A2 ->
+   eq_type A2 A1
+| EqTransType : forall A1 A2 A3,
+   eq_type A1 A2 ->
+   eq_type A2 A3 ->
+   eq_type A1 A3
+(** Enforce compatibility with substitution **)
+| EqSubstIdType : forall {ctx : wfCtx} (A : @wfType ctx),
+   eq_type (TSubst ctx A (Id ctx)) (A)
+| EqSubstCompType : forall {Delta mid Gamma : wfCtx}
+(A : @wfType Gamma) (g1 : @wfSub Delta mid) (g0 : @wfSub mid Gamma),
+   eq_type (TSubst Delta A (g0 ∘ g1)) (TSubst mid (TSubst Gamma A g0) g1)
+.
+
+Definition TypeEqJG {ctx : wfCtx} : relation (@wfType ctx) := eq_type.
+Lemma TypeEqJG_refl {ctx : wfCtx} (A : @wfType ctx) :
+    TypeEqJG A A.
+Proof.
+   constructor.
+Qed.
+Lemma TypeEqJG_sym {ctx : wfCtx} (A1 A2 : @wfType ctx) :
+   TypeEqJG A1 A2  ->
+   TypeEqJG A2 A1.
+Proof.
+   constructor.
+   exact H.
+Qed.
+Lemma TypeEqJG_trans {ctx : wfCtx} (A1 A2 A3 : @wfType ctx) :
+   TypeEqJG A1 A2 ->
+   TypeEqJG A2 A3 ->
+   TypeEqJG A1 A3.
+Proof.
+   apply EqTransType.
+Qed.
+
+Add Parametric Relation (ctx :wfCtx) : (@wfType ctx) (@TypeEqJG ctx)
+   reflexivity proved by (@TypeEqJG_refl ctx)
+   symmetry proved by (@TypeEqJG_sym ctx)
+   transitivity proved by (@TypeEqJG_trans ctx)
+   as TypeEqJG_rel.
+
+Notation "[ ctx ⊢ A1 '==' A2 ]" := (@TypeEqJG ctx A1 A2) (at level 50).
+
+(*** End Equality for Types ***)
+
+
+(*** Equality for Terms ***)
+Inductive eq_term : relation preTerm :=
+(** Enforce equivalence **)
+| EqReflTerm : forall t, eq_term t t
+| EqSymTerm : forall t1 t2,
+   eq_term t1 t2 ->
+   eq_term t2 t1
+| EqTransTerm : forall t1 t2 t3,
+   eq_term t1 t2 ->
+   eq_term t2 t3 ->
+   eq_term t1 t3
+(** Enforce compatibility with substitution **)
+| EqSubstIdTerm: forall {ctx : wfCtx} {A : @wfType ctx} (a : @wfTerm ctx A),
+   eq_term (ESubst ctx A a ctx (Id ctx)) (a)
+| EqSubstCompTerm : forall {Delta mid Gamma : wfCtx}
+   {A : @wfType Gamma} (a : @wfTerm Gamma A)
+   (g1 : @wfSub Delta mid) (g0 : @wfSub mid Gamma),
+      eq_term (ESubst Delta A a Gamma (g0 ∘ g1)) (ESubst Delta (TSubst Gamma A g0) (ESubst mid A a Gamma g0) mid g1)
+.
+Definition TermEqJG {ctx : wfCtx} {A : @wfType ctx} : relation (@wfTerm ctx A) := eq_term.
+Lemma TermEqJG_refl {ctx : wfCtx} {A : @wfType ctx} (t : @wfTerm ctx A) :
+    TermEqJG t t.
+Proof.
+   constructor.
+Qed.
+Lemma TermEqJG_sym {ctx : wfCtx} {A : @wfType ctx} (t1 t2 : @wfTerm ctx A) :
+   TermEqJG t1 t2  ->
+   TermEqJG t2 t1.
+Proof.
+   constructor.
+   exact H.
+Qed.
+Lemma TermEqJG_trans {ctx : wfCtx} {A : @wfType ctx} (t1 t2 t3 : @wfTerm ctx A) :
+   TermEqJG t1 t2 ->
+   TermEqJG t2 t3 ->
+   TermEqJG t1 t3.
+Proof.
+   apply EqTransTerm.
+Qed.
+
+Add Parametric Relation (ctx :wfCtx) (A : @wfType ctx) : (@wfTerm ctx A) (@TermEqJG ctx A)
+   reflexivity proved by (@TermEqJG_refl ctx A)
+   symmetry proved by (@TermEqJG_sym ctx A)
+   transitivity proved by (@TermEqJG_trans ctx A)
+   as TermEqJG_rel.
+Notation "[ ctx ⊢ t1 '==' t2 ; A ]" := (@TermEqJG ctx A t1 t2) (at level 50).
+
+(*** End Equality for Terms ***)
+
+(** End Equality Judgements **)
+
+
